a = b<sup>y</b>

16 = 2<sup>?</sup>

y = log<sub>b</sub>(a)

? = log<sub>5</sub>(25) = 2

? = log<sub>2</sub>(16) = 4

a = b<sup>y</sup>

log(a) = y log(b)

y = log<sub>b</sub>(a) = log(a) / log(b)

log<sub>5</sub>(25) = log(25) / log(5)


T = 2 * T(n/2) + n

T = 2 * (2 * T(n/4) + n) + n

T = 4 * T(n/4) + 2 * n + n
T = 8 * T(n/8) + 4*n + 2*n + n

n = 2<sup>k</sup>

k = log<sub>2</sub>(n)
T = n + 2n + 4n + ... + log(n) * n
  = n (1 + 2 + 4 + ... + log(n))

  = n (log(n)<sup>log(n)</sup> - 1)







